src/Set_Proc_Code.thy
@@ -1,6 +1,13 @@
 theory Set_Proc_Code
-  imports Set_Proc
+  imports Set_Proc Typing_Urelems "Fresh_Identifiers.Fresh_Nat" "List-Index.List_Index"
 begin
+
+instantiation nat :: default
+begin
+definition "default_nat = (0::nat)"
+
+instance ..
+end
 
 fun subterms_term_list :: "'a pset_term \<Rightarrow> 'a pset_term list"  where
   "subterms_term_list (\<emptyset> n) = [\<emptyset> n]"
@@ -251,5 +258,327 @@ lemma lexpands_if_lexpand:
   using lexpands_single_if_lexpand_single lexpands_eq_if_lexpand_eq
   using lexpands.intros by fastforce
 
+fun bexpand_nowit1 :: "'a branch \<Rightarrow> 'a pset_fm \<Rightarrow> 'a branch list list" where
+  "bexpand_nowit1 b (Or p q) =
+    (if p \<notin> set b \<and> Neg p \<notin> set b then [[[p], [Neg p]]] else [])"
+| "bexpand_nowit1 b (Neg (And p q)) =
+    (if Neg p \<notin> set b \<and> p \<notin> set b then [[[Neg p], [p]]] else [])"
+| "bexpand_nowit1 b (AT (s \<in>\<^sub>s t)) =
+    [[[AT (s \<in>\<^sub>s t2)], [AF (s \<in>\<^sub>s t2)]]. t' \<sqinter>\<^sub>s t2 \<leftarrow> subterms_fm_list (last b), t' = t,
+                                       AT (s \<in>\<^sub>s t2) \<notin> set b, AF (s \<in>\<^sub>s t2) \<notin> set b] @
+    [[[AT (s \<in>\<^sub>s t2)], [AF (s \<in>\<^sub>s t2)]]. t' -\<^sub>s t2 \<leftarrow> subterms_fm_list (last b), t' = t,
+                                       AT (s \<in>\<^sub>s t2) \<notin> set b, AF (s \<in>\<^sub>s t2) \<notin> set b] @
+    (case t of
+      t1 \<squnion>\<^sub>s t2 \<Rightarrow>
+        (if t1 \<squnion>\<^sub>s t2 \<in> subterms (last b) \<and> AT (s \<in>\<^sub>s t1) \<notin> set b \<and> AF (s \<in>\<^sub>s t1) \<notin> set b
+          then [[[AT (s \<in>\<^sub>s t1)], [AF (s \<in>\<^sub>s t1)]]] else [])
+    | _ \<Rightarrow> [])"
+| "bexpand_nowit1 b _ = []"
+
+definition "bexpand_nowit b \<equiv> concat (map (bexpand_nowit1 b) b)"
+
+lemma bexpand_nowit_if_bexpands_nowit:
+  "bexpands_nowit bs' b \<Longrightarrow> bs' \<in> set ` set (bexpand_nowit b)"
+  apply(induction rule: bexpands_nowit.induct)
+       apply(force simp: bexpand_nowit_def)+
+  done
+
+lemma bexpands_nowit_if_bexpand_nowit1:
+  "bs' \<in> set ` set (bexpand_nowit1 b l) \<Longrightarrow> l \<in> set b \<Longrightarrow> bexpands_nowit bs' b"
+  apply(induction b l rule: bexpand_nowit1.induct)
+          apply(auto simp: bexpands_nowit.intros)
+  done
+
+lemma bexpands_nowit_if_bexpand_nowit:
+  "bs' \<in> set ` set (bexpand_nowit b) \<Longrightarrow> bexpands_nowit bs' b"
+  unfolding bexpand_nowit_def using bexpands_nowit_if_bexpand_nowit1
+  by (auto simp: bexpands_nowit.intros)
+
+definition "name_subterm \<phi> \<equiv> index (subterms_fm_list \<phi>)"
+
+lemma inj_on_name_subterm_subterms:
+  "inj_on (name_subterm \<phi>) (subterms \<phi>)"
+  unfolding name_subterm_def
+  by (intro inj_on_index2) simp
+
+abbreviation "solve_constraints \<phi> \<equiv>
+  Suc_Theory.solve (Suc_Theory.elim_NEq_Zero (constrs_fm (name_subterm \<phi>) \<phi>))"
+
+definition "urelem_code \<phi> t \<equiv>
+  (case solve_constraints \<phi> of
+    Some ss \<Rightarrow> Suc_Theory.assign ss (name_subterm \<phi> t) = 0
+  | None \<Rightarrow> False)"
+
+lemma urelem_code_if_mem_subterms:
+  assumes "t \<in> subterms \<phi>"
+  shows "urelem \<phi> t \<longleftrightarrow> urelem_code \<phi> t"
+proof -
+  note urelem_iff_assign_eq_0[OF _ assms] not_types_fm_if_solve_eq_None
+  note solve_correct = this[OF inj_on_name_subterm_subterms]
+  then show ?thesis
+    unfolding urelem_def urelem_code_def
+    by (auto split: option.splits)
+qed
+
+fun bexpand_wit1 :: "('a::{fresh,default}) branch \<Rightarrow> 'a pset_fm \<Rightarrow> 'a branch list list" where
+  "bexpand_wit1 b (AF (t1 =\<^sub>s t2)) =
+    (if t1 \<in> subterms (last b) \<and> t2 \<in> subterms (last b) \<and>
+        (\<forall>t \<in> set b. case t of AT (x \<in>\<^sub>s t1') \<Rightarrow> t1' = t1 \<longrightarrow> AF (x \<in>\<^sub>s t2) \<notin> set b | _ \<Rightarrow> True) \<and>
+        (\<forall>t \<in> set b. case t of AT (x \<in>\<^sub>s t2') \<Rightarrow> t2' = t2 \<longrightarrow> AF (x \<in>\<^sub>s t1) \<notin> set b | _ \<Rightarrow> True) \<and>
+        \<not> urelem_code (last b) t1 \<and> \<not> urelem_code (last b) t2
+      then
+        (let x = fresh (vars b) default
+         in [[[AT (Var x \<in>\<^sub>s t1), AF (Var x \<in>\<^sub>s t2)],
+              [AT (Var x \<in>\<^sub>s t2), AF (Var x \<in>\<^sub>s t1)]]])
+      else [])"
+| "bexpand_wit1 b _ = []"
+
+definition "bexpand_wit b \<equiv> concat (map (bexpand_wit1 b) b)"
+
+lemma Not_Ex_wit_code:
+  "(\<nexists>x. AT (x \<in>\<^sub>s t1) \<in> set b \<and> AF (x \<in>\<^sub>s t2) \<in> set b)
+    \<longleftrightarrow> (\<forall>fm \<in> set b. case fm of
+                        AT (x \<in>\<^sub>s t') \<Rightarrow> t' = t1 \<longrightarrow> AF (x \<in>\<^sub>s t2) \<notin> set b
+                      | _ \<Rightarrow> True)"
+  by (auto split: fm.splits pset_atom.splits)
+
+lemma bexpand_wit1_if_bexpands_wit:
+  assumes "bexpands_wit t1 t2 (fresh (vars b) default) bs' b"
+  shows "bs' \<in> set ` set (bexpand_wit1 b (AF (t1 =\<^sub>s t2)))"
+proof -
+  from bexpands_witD[OF assms] show ?thesis
+    by (simp add: Let_def urelem_code_if_mem_subterms Not_Ex_wit_code[symmetric])
+qed
+
+lemma bexpand_wit_if_bexpands_wit:
+  assumes "bexpands_wit t1 t2 (fresh (vars b) default) bs' b"
+  shows "bs' \<in> set ` set (bexpand_wit b)"
+  using assms(1)[THEN bexpand_wit1_if_bexpands_wit] bexpands_witD(2)[OF assms(1)]
+  unfolding bexpand_wit_def 
+  by (auto simp del: bexpand_wit1.simps(1))
+  
+lemma bexpands_wit_if_bexpand_wit1:
+  "b' \<in> set ` set (bexpand_wit1 b l) \<Longrightarrow> l \<in> set b \<Longrightarrow> (\<exists>t1 t2 x. bexpands_wit t1 t2 x b' b)"
+proof(induction b l rule: bexpand_wit1.induct)
+  case (1 b t1 t2)
+  show ?case
+    apply(rule exI[where ?x=t1], rule exI[where ?x=t2],
+          rule exI[where ?x="fresh (vars b) default"])
+    using 1
+    by (auto simp: Let_def bexpands_wit.simps finite_vars_branch[THEN fresh_notIn]
+                   Not_Ex_wit_code[symmetric] urelem_code_if_mem_subterms)
+qed auto
+    
+lemma bexpands_wit_if_bexpand_wit:
+  "bs' \<in> set ` set (bexpand_wit b) \<Longrightarrow> (\<exists>t1 t2 x. bexpands_wit t1 t2 x bs' b)"
+  using bexpands_wit_if_bexpand_wit1[of bs' b]
+  apply auto
+  using bexpands_wit.intros
+  sorry
+                                
+definition "bexpand b \<equiv> bexpand_nowit b @ bexpand_wit b"
+
+lemma bexpands_if_bexpand:
+  "bs' \<in> set ` set (bexpand b) \<Longrightarrow> bexpands bs' b"
+  unfolding bexpand_def
+  using bexpands_nowit_if_bexpand_nowit bexpands_wit_if_bexpand_wit
+  using bexpands.simps by fastforce
+
+lemma Not_bexpands_if_bexpand_empty:
+  assumes "bexpand b = []"
+  shows "\<not> bexpands bs' b"
+proof
+  assume "bexpands bs' b"
+  then show False
+    using assms
+  proof (induction rule: bexpands.induct)
+    case (1 bs' b)
+    with bexpand_nowit_if_bexpands_nowit[OF this(1)] show ?case
+      unfolding bexpand_def by simp
+  next
+    case (2 t1 t2 x bs' b)
+    with bexpand_wit_if_bexpands_wit bexpands_witD[OF this(1)] show ?case
+      using fresh_notIn[OF finite_vars_branch, of b]
+      unfolding bexpand_def
+      by (metis Nil_is_append_conv bexpands_wit.intros empty_iff empty_set)
+     
+  qed
+qed
+
+lemma lin_sat_code:
+  "lin_sat b \<longleftrightarrow> filter (\<lambda>b'. \<not> set b' \<subseteq> set b) (lexpand b) = []"
+  unfolding lin_sat_def
+  using lexpand_if_lexpands lexpands_if_lexpand
+  by (force simp: filter_empty_conv)
+
+lemma sat_code:
+  "sat b \<longleftrightarrow> lin_sat b \<and> bexpand b = []"
+  by (meson Not_bexpands_if_bexpand_empty bexpands_if_bexpand last_in_set sat_def)
+
+fun bclosed_code1 :: "'a branch \<Rightarrow> 'a pset_fm \<Rightarrow> bool" where
+  "bclosed_code1 b (Neg \<phi>) \<longleftrightarrow>
+    \<phi> \<in> set b \<or>
+    (case \<phi> of Atom (t1 =\<^sub>s t2) \<Rightarrow> t1 = t2 | _ \<Rightarrow> False)"
+| "bclosed_code1 b (AT (_ \<in>\<^sub>s \<emptyset> _)) \<longleftrightarrow> True"
+| "bclosed_code1 _ _ \<longleftrightarrow> False"
+
+definition "bclosed_code b \<equiv> (\<exists>t \<in> set b. bclosed_code1 b t)"
+
+lemma bclosed_code_if_bclosed:
+  assumes "bclosed b" "wf_branch b" "v \<turnstile> last b"
+  shows "bclosed_code b"
+  using assms
+proof(induction rule: bclosed.induct)
+  case (contr \<phi> b)
+  then have "bclosed_code1 b (Neg \<phi>)"
+    by auto
+  with contr show ?case
+    unfolding bclosed_code_def by blast
+next
+  case (memEmpty t n b)
+  then have "bclosed_code1 b (AT (t \<in>\<^sub>s \<emptyset> n))"
+    by auto
+  with memEmpty show ?case
+    unfolding bclosed_code_def by blast
+next
+  case (neqSelf t b)
+  then have "bclosed_code1 b (AF (t =\<^sub>s t))"
+    by auto
+  with neqSelf show ?case
+    unfolding bclosed_code_def by blast
+next
+  case (memberCycle cs b)
+  then show ?case
+    by (auto simp: bclosed_code_def dest: no_member_cycle_if_types_last)
+qed
+
+lemma bclosed_if_bclosed_code1:
+  "bclosed_code1 b l \<Longrightarrow> l \<in> set b \<Longrightarrow> bclosed b"
+  by (induction rule: bclosed_code1.induct)
+     (auto simp: bclosed.intros split: fm.splits pset_atom.splits)
+
+lemma bclosed_if_bclosed_code:
+  "bclosed_code b \<Longrightarrow> bclosed b"
+  unfolding bclosed_code_def using bclosed_if_bclosed_code1 by blast
+
+lemma bclosed_code:
+  assumes "wf_branch b" "v \<turnstile> last b"
+  shows "bclosed b \<longleftrightarrow> bclosed_code b"
+  using assms bclosed_if_bclosed_code bclosed_code_if_bclosed 
+  by blast
+
+definition "lexpand_safe b \<equiv>
+  case filter (\<lambda>b'. \<not> set b' \<subseteq> set b) (lexpand b) of
+    b' # bs' \<Rightarrow> b'
+  | [] \<Rightarrow> []"
+
+lemma lexpands_lexpand_safe:
+  "\<not> lin_sat b \<Longrightarrow> lexpands (lexpand_safe b) b \<and> set b \<subset> set (lexpand_safe b @ b)"
+  unfolding lexpand_safe_def
+  by (auto simp: lin_sat_code intro!: lexpands_if_lexpand dest: filter_eq_ConsD split: list.splits)
+
+
+lemma wf_branch_lexpand_safe:
+  assumes "wf_branch b"
+  shows "wf_branch (lexpand_safe b @ b)"
+proof -
+  from assms have "wf_branch (lexpand_safe b @ b)" if "\<not> lin_sat b"
+    using that lexpands_lexpand_safe wf_branch_lexpands by metis
+  moreover have "wf_branch (lexpand_safe b @ b)" if "lin_sat b"
+    using assms that[unfolded lin_sat_code]
+    unfolding lexpand_safe_def by simp
+  ultimately show ?thesis
+    by blast
+qed
+
+definition "bexpand_safe b \<equiv>
+  case bexpand b of
+    bs' # bss' \<Rightarrow> bs'
+  | [] \<Rightarrow> {[]}"
+
+lemma bexpands_bexpand_safe:
+  "\<not> sat b \<Longrightarrow> lin_sat b \<Longrightarrow> bexpands (bexpand_safe b) b"
+  unfolding bexpand_safe_def
+  by (auto simp: sat_code bexpands_if_bexpand split: list.splits)
+
+lemma wf_branch_bexpand_safe:
+  assumes "wf_branch b"
+  shows "\<forall>b' \<in> bexpand_safe b. wf_branch (b' @ b)"
+proof -
+  note wf_branch_expandss[OF assms expandss.intros(3), OF bexpands_if_bexpand]
+  with assms show ?thesis
+    unfolding bexpand_safe_def
+    by (simp split: list.splits) (metis expandss.intros(1) list.set_intros(1))
+qed
+
+global_interpretation mlss_naive: mlss_proc lexpand_safe bexpand_safe
+  apply(unfold_locales)
+  using lexpands_lexpand_safe bexpands_bexpand_safe by auto
+
+
+lemma types_pset_fm_code:
+  "(\<exists>v. v \<turnstile> \<phi>) \<longleftrightarrow> solve_constraints \<phi> \<noteq> None"
+  using not_types_fm_if_solve_eq_None types_pset_fm_assign_solve
+  by (meson inj_on_name_subterm_subterms not_Some_eq)
+
+typedef 'a wf_branch = "{b :: 'a branch. wf_branch b \<and> (\<exists>v. v \<turnstile> last b)}"
+proof -
+  have types: "(\<lambda>_. 0) \<turnstile> AT (\<emptyset> 0 =\<^sub>s \<emptyset> 0)"
+    unfolding types_pset_fm_def 
+    by (auto intro!: types_pset_atom.intros types_pset_term.intros)
+  show ?thesis
+    apply(rule exI[where ?x="[AT (\<emptyset> 0 =\<^sub>s \<emptyset> 0)]"])
+    using types wf_branch_singleton by auto
+qed
+setup_lifting type_definition_wf_branch
+
+lift_definition lin_sat_wf :: "'a wf_branch \<Rightarrow> bool" is lin_sat .
+lift_definition sat_wf :: "'a wf_branch \<Rightarrow> bool" is sat .
+
+lemma lin_sat_wf_code[code]:
+  "lin_sat_wf b
+  \<longleftrightarrow> filter (\<lambda>b'. \<not> set b' \<subseteq> set (Rep_wf_branch b)) (lexpand (Rep_wf_branch b)) = []"
+  by transfer (use lin_sat_code in blast)
+
+lemma sat_wf_code[code]:
+  "sat_wf b \<longleftrightarrow> lin_sat_wf b \<and> bexpand (Rep_wf_branch b) = []"
+  by transfer (use sat_code in blast)
+
+lift_definition bclosed_wf :: "'a wf_branch \<Rightarrow> bool" is bclosed .
+lift_definition bclosed_code_wf :: "'a wf_branch \<Rightarrow> bool" is bclosed_code .
+
+lemma bclosed_wf_code[code]:
+  "bclosed_wf b = bclosed_code_wf b"
+  by transfer (use bclosed_code in blast)
+
+lift_definition lexpand_safe_app_wf :: "'a wf_branch \<Rightarrow> 'a wf_branch"
+  is "\<lambda>b. lexpand_safe b @ b"
+  using wf_branch_lexpand_safe by auto
+
+lift_definition bexpand_safe_app_wf :: "('a::{fresh,default}) wf_branch \<Rightarrow> 'a wf_branch set"
+  is "\<lambda>b. (\<lambda>b'. b' @ b) ` bexpand_safe b"
+  using wf_branch_bexpand_safe by auto
+
+lift_definition mlss_proc_branch_wf :: "('a::{fresh,default}) wf_branch \<Rightarrow> bool"
+  is "mlss_naive.mlss_proc_branch" .
+
+lemma mlss_proc_branch_wf_code[code]:
+  "mlss_proc_branch_wf b =
+    (if \<not> lin_sat_wf b then mlss_proc_branch_wf (lexpand_safe_app_wf b)
+     else if bclosed_wf b then True
+     else if \<not> sat_wf b then (\<forall>b' \<in> bexpand_safe_app_wf b. mlss_proc_branch_wf b')
+     else bclosed_wf b)"
+  apply transfer
+  apply (auto simp: mlss_naive.mlss_proc_branch_dom_if_wf_branch
+                    mlss_naive.mlss_proc_branch.psimps)
+  done
+
+lemma Ball_bexpand_safe_app_wf[code_unfold]:
+  "(\<forall>b' \<in> bexpand_safe_app_wf b. mlss_proc_branch_wf b')
+  \<longleftrightarrow> (\<forall>b' \<in> bexpand_safe (Rep_wf_branch b). mlss_proc_branch_wf (Abs_wf_branch (b' @ b))"
+  sorry
+
+code_identifier code_module Set_Calculus \<rightharpoonup> (SML) Set_Proc_Code
+export_code mlss_proc_branch_wf in SML
 
 end
